execution/examples/Cis1wccd.v
@@ -1,0 +1,481 @@
+(**
+  This file contains an implementation of the example token that complies with the Concordium's CIS1 standard.
+  The development is inspired by the Rust implementation: https://github.com/Concordium/concordium-rust-smart-contracts/tree/main/examples/cis1-wccd
+*)
+
+From Coq Require Import ZArith.
+From Coq Require Import List.
+From ConCert.Execution Require Import Monads.
+From ConCert.Execution Require Import Containers.
+From ConCert.Execution Require Import Extras.
+From ConCert.Execution Require Import Serializable.
+From ConCert.Execution Require Import Blockchain.
+From ConCert.Execution.Examples Require Import Common.
+From ConCert.Execution.Standards.CIS1 Require Import CIS1Spec.
+From ConCert.Utils Require Import RecordUpdate.
+
+Import ListNotations.
+Import RecordSetNotations.
+
+Definition requireTrue (cond : bool) :=
+  if cond then Some tt else None.
+
+Section WccdToken.
+  Context {BaseTypes : ChainBase}.
+  Set Nonrecursive Elimination Schemes.
+
+  Definition TOKEN_ID_WCCD : TokenID := 0.
+
+  Open Scope bool.
+
+  (** * Entry points *)
+
+  Record wccd_transfer_params :=
+    { wccd_td_amount   : TokenAmount;
+      wccd_td_from     : Address;
+      wccd_td_to       : Address }.
+
+  Inductive OpUpdateKind :=
+    opAdd
+  | opDelete.
+
+  Inductive Msg :=
+  | wccd_msg_transfer (params : list wccd_transfer_params)
+  | wccd_msg_balanceOf (query : list Address)
+                   (send_results_to : Address)
+  | wccd_msg_updateOperator (params : list (OpUpdateKind * Address))
+  | wccd_msg_mint (receiver : Address)
+  | wccd_msg_burn (amount : TokenAmount).
+
+  (** * Contract's state *)
+  (** The state tracked for each address.*)
+  Record AddressState := {
+        wccd_balance:   TokenAmount;
+        wccd_operators: list Address
+    }.
+
+  (* begin hide *)
+  MetaCoq Run (make_setters AddressState).
+  (* end hide *)
+
+
+  (** The contract state: a mapping from addresses to [AddressState] *)
+
+  Definition State := AddressMap.AddrMap AddressState.
+
+  Section Serialization.
+
+    Global Instance OpUpdateKind_serializable : Serializable OpUpdateKind :=
+      Derive Serializable OpUpdateKind_rect <opAdd, opDelete>.
+
+    Global Instance state_serializable : Serializable AddressState :=
+      Derive Serializable AddressState_rect <Build_AddressState>.
+
+    Global Instance wccd_transfer_params_serializable : Serializable wccd_transfer_params :=
+      Derive Serializable wccd_transfer_params_rect <Build_wccd_transfer_params>.
+
+    Global Instance msg_serializable : Serializable Msg :=
+      Derive Serializable Msg_rect <wccd_msg_transfer, wccd_msg_balanceOf, wccd_msg_updateOperator, wccd_msg_mint, wccd_msg_burn>.
+
+  End Serialization.
+
+  (** Transfer *)
+
+  Definition increment_balance (st : State) (addr : Address) (inc : TokenAmount) : State :=
+    match AddressMap.find addr st with
+    | Some old => AddressMap.add addr (old<| wccd_balance := old.(wccd_balance) + inc |>) st
+    | None => AddressMap.add addr {| wccd_balance := inc
+                                   ; wccd_operators := [] |} st
+    end.
+
+  Definition decrement_balance (st : State) (addr : Address) (dec : TokenAmount) : option State :=
+    do old <- AddressMap.find addr st;
+    let old_balance := old.(wccd_balance) in
+    do requireTrue (dec <=? old_balance);
+    ret (AddressMap.add addr (old<| wccd_balance := old_balance - dec |>) st).
+
+  (** Single transfer of [amount] between [from] and [to] *)
+  Definition wccd_transfer_single
+             (token_id : TokenID)
+             (amount : TokenAmount)
+             (from to : Address)
+             (prev_st : State) : option State :=
+    do requireTrue (token_id =? TOKEN_ID_WCCD);
+    do st <- decrement_balance prev_st from amount;
+    ret (increment_balance st to amount).
+
+  (** Batch execution of all transfers in the list. Note that the
+      operation succeeds only if all transfers in the batch succeed *)
+  Definition wccd_transfer (transfers : list wccd_transfer_params) (prev_st : State)
+    : option State :=
+    monad_foldl (fun acc x =>
+                   wccd_transfer_single TOKEN_ID_WCCD x.(wccd_td_amount) x.(wccd_td_from) x.(wccd_td_to) acc)
+                prev_st transfers.
+
+  (** * balanceOf *)
+
+  Definition get_balance_opt (addr : Address) (st : State) : option TokenAmount :=
+    match AddressMap.find addr st with
+    | Some data => Some data.(wccd_balance)
+    | None => None
+    end.
+
+  Definition wccd_balanceOf (query : list Address) (st : State)
+    : list (TokenID * Address * TokenAmount) :=
+    map (fun addr => (TOKEN_ID_WCCD, addr, with_default TOKEN_ID_WCCD (get_balance_opt addr st))) query.
+
+  (** * updateOperator *)
+
+  Definition add_remove (param : OpUpdateKind * Address) (operators : list Address) :=
+    let '(updateKind,addr) := param in
+    match updateKind with
+    | opAdd => addr :: operators
+    | opDelete => remove address_eqdec addr operators
+    end.
+
+  Definition wccd_updateOperator (owner : Address) (params : list (OpUpdateKind * Address)) (prev_st : State)
+    : option State :=
+    (* NOTE: in contrast to the Concordium's implementation, we do not
+       allow to add operators to non-existing addresses *)
+    do owner_data <- AddressMap.find owner prev_st;
+    let updated_owner_data := owner_data<| wccd_operators := fold_right add_remove owner_data.(wccd_operators) params |> in
+    ret (AddressMap.add owner updated_owner_data prev_st).
+
+  (** * Wccd receive *)
+
+  (* We dispatch on a message of type [Msg] and call the corresponding functions with received parameters *)
+  Definition wccd_receive (chain : Chain) (ctx : ContractCallContext) (prev_st : State) (msg : option Msg) :
+    option (State * list ActionBody) :=
+    match msg with
+    | Some (wccd_msg_transfer params) =>
+        do next_st <- wccd_transfer params prev_st;
+        let contract_accounts := filter (fun x => address_is_contract x.(wccd_td_to)) params in
+        let mk_callback_data x :=
+          serialize
+            (CIS1_receiver_receive_hook unit
+            (TOKEN_ID_WCCD,x.(wccd_td_amount), x.(wccd_td_from))) in
+        let ops := map (fun x => act_call x.(wccd_td_to) 0 (mk_callback_data x)) contract_accounts in
+        ret (next_st, ops)
+    | Some (wccd_msg_balanceOf query send_to) =>
+        let balances := wccd_balanceOf query prev_st in
+        do requireTrue (address_is_contract send_to);
+        ret (prev_st, [act_call send_to 0 (serialize balances)])
+    | Some (wccd_msg_updateOperator params) =>
+        do next_st <- wccd_updateOperator ctx.(ctx_from) params prev_st;
+        ret (next_st, [])
+    | Some (wccd_msg_mint receiver) =>
+        (** Check that the sender is not the receiver *)
+        do requireTrue (negb (address_eqb receiver ctx.(ctx_from)));
+        let next_st := increment_balance prev_st receiver (Z.to_nat ctx.(ctx_amount)) in
+        (** NOTE: we only update the state and do not notify the receiver *)
+        ret (next_st,[])
+    | Some (wccd_msg_burn amt) =>
+        (** Check that the sender is not the receiver *)
+        do next_st <- decrement_balance prev_st ctx.(ctx_from) amt;
+        ret (next_st, [act_transfer ctx.(ctx_from) (Z.of_nat amt)])
+    | None => None
+    end.
+
+End WccdToken.
+
+(** * Wccd token complies with CIS1 *)
+
+Module WccdTypes <: CIS1Types.
+
+  Definition Msg `{ChainBase} := Msg.
+
+  Definition Storage `{ChainBase} := State.
+
+End WccdTypes.
+
+Module WccdView <: CIS1View WccdTypes.
+
+  Import WccdTypes.
+
+  Section WccdViewDefs.
+
+    Context `{ChainBase}.
+
+    Definition get_balance_opt st (token_id : TokenID) addr :=
+      do requireTrue (token_id =? TOKEN_ID_WCCD);
+      get_balance_opt addr st.
+
+    Definition get_operators (st : Storage) (addr : Address) :=
+      match AddressMap.find addr st with
+      | Some v => v.(wccd_operators)
+      | None => []
+      end.
+
+    Definition get_owners : Storage -> TokenID -> list Address :=
+      fun st token_id => if (token_id =? TOKEN_ID_WCCD) then
+                           FMap.keys st
+                         else [].
+
+    Lemma get_owners_no_dup : forall st token_id, NoDup (get_owners st token_id).
+    Proof.
+      intros. unfold get_owners.
+      destruct (_ =? _);[apply FMap.NoDup_keys | constructor ].
+    Qed.
+
+    Lemma In_keys_In_elements_iff {K V : Type} `{countable.Countable K} (m : FMap K V) (k : K) :
+      In k (FMap.keys m) <-> exists v, In (k,v) (FMap.elements m).
+    Proof.
+      split.
+      - induction m using fin_maps.map_ind; intros Hin.
+        + easy.
+        + unfold FMap.keys in *.
+          rewrite FMap.elements_add in Hin by assumption.
+          cbn in *. destruct Hin.
+          * exists x. rewrite FMap.elements_add by assumption. now left.
+          * destruct (IHm H2) as [x0 Hx0]. exists x0.
+            rewrite FMap.elements_add by assumption.
+            now right.
+      - induction m using fin_maps.map_ind; intros Hex.
+        + now destruct Hex.
+        + destruct Hex as [v Hv].
+          unfold FMap.keys.
+          rewrite FMap.elements_add in * by assumption;cbn in *.
+          destruct Hv as [HH | HH];try inversion HH;easy.
+    Qed.
+
+    Lemma get_owners_balances : forall st owner token_id,
+        In owner (get_owners st token_id) <->
+          exists balance, get_balance_opt st token_id owner = Some balance.
+    Proof.
+      split.
+      + intros Hin. unfold get_owners in *.
+        unfold get_balance_opt,Cis1wccd.get_balance_opt.
+        destruct (_ =? _);try inversion Hin.
+        apply In_keys_In_elements_iff in Hin.
+        destruct Hin as [a_st HH].
+        exists a_st.(wccd_balance).
+        apply FMap.In_elements in HH.
+        unfold AddressMap.find,FMap.find in *.
+        now rewrite HH.
+      + intros Hex.
+        destruct Hex as [b Hb].
+        unfold get_owners, FMap.keys.
+        unfold get_balance_opt,Cis1wccd.get_balance_opt in *.
+        destruct (_ =? _);try inversion Hb.
+        destruct (AddressMap.find owner st) eqn:Heq;try congruence.
+        unfold AddressMap.find in *.
+        apply FMap.In_elements in Heq.
+        apply In_keys_In_elements_iff.
+        eauto.
+    Qed.
+
+    Definition token_id_exists (st : Storage) (token_id : TokenID) : bool :=
+      token_id =? TOKEN_ID_WCCD.
+
+
+  End WccdViewDefs.
+End WccdView.
+
+Module WccdReceiveSpec <: CIS1ReceiveSpec WccdTypes WccdView.
+
+  Module cis1_axioms := CIS1Axioms WccdTypes WccdView.
+  Import cis1_axioms.
+
+  Module BalancesFacts := CIS1Balances WccdTypes WccdView.
+  Import BalancesFacts.
+
+  Section WccdReceiveDefs.
+
+    Context `{ChainBase}.
+
+    Definition to_cis1_transfer_data (p : wccd_transfer_params) : CIS1_transfer_data :=
+      let '(Build_wccd_transfer_params amt from_addr to_addr) := p in
+      {| cis1_td_token_id := TOKEN_ID_WCCD;
+         cis1_td_amount := amt;
+         cis1_td_from := from_addr;
+        cis1_td_to := to_addr |}.
+
+    Definition to_cis1_updateOperator_kind (op : OpUpdateKind) : CIS1_updateOperator_kind :=
+      match op with
+      | opAdd => cis1_ou_add_operator
+      | opDelete => cis1_ou_remove_operator
+      end.
+
+    Definition to_cis1_balanceOf_params (query : list Address) (send_to : Address)
+      : option CIS1_balanceOf_params :=
+      match Bool.bool_dec (address_is_contract send_to) true with
+      | left p =>
+          Some {|cis1_bo_query := map (fun addr => Build_CIS1_balanceOf_query _ TOKEN_ID_WCCD addr) query;
+                 cis1_bo_result_address := send_to;
+                 cis1_bo_result_address_is_contract := p |}
+      | right _ => None
+      end.
+
+    Definition get_CIS1_entry_point : Msg -> option CIS1_entry_points :=
+      fun msg => match msg with
+              | wccd_msg_transfer params =>
+                  let params :=
+                    {| cis_tr_transfers := map to_cis1_transfer_data params|} in
+                  Some (CIS1_transfer params)
+              | wccd_msg_balanceOf query send_results_to =>
+                  do p <- to_cis1_balanceOf_params query send_results_to;
+                  Some (CIS1_balanceOf p)
+              | wccd_msg_updateOperator params =>
+                  let upd_list :=
+                    map (fun '(upd_kind, addr) =>
+                           Build_CIS1_updateOperator_update _ (to_cis1_updateOperator_kind upd_kind) addr) params in
+                  Some (CIS1_updateOperator {| cis1_ou_params := upd_list |})
+              | wccd_msg_mint receiver => None
+              | wccd_msg_burn amount => None
+              end.
+
+    Definition get_contract_msg :  CIS1_entry_points -> Msg.
+    Admitted.
+
+    Lemma left_inverse_get_CIS1_entry_point (entry_point : CIS1_entry_points) :
+      get_CIS1_entry_point (get_contract_msg entry_point) = Some entry_point.
+    Proof.
+      Admitted.
+
+    Lemma inctement_balance_find_ne st addr1 addr2 amt :
+      addr1 <> addr2 ->
+      AddressMap.find addr1 (increment_balance st addr2 amt) = AddressMap.find addr1 st.
+    Proof.
+      intros Hneq.
+      unfold increment_balance.
+      destruct (AddressMap.find addr2 _);
+        unfold AddressMap.add, AddressMap.find;
+        now rewrite fin_maps.lookup_insert_ne.
+    Qed.
+
+    Import Lia.
+
+    Lemma wccd_transfer_single_cis1 (amt : TokenAmount) (from_addr to_addr : Address)
+          (prev_st st : State) :
+        wccd_transfer_single TOKEN_ID_WCCD amt from_addr to_addr prev_st = Some st ->
+        transfer_single_spec prev_st st TOKEN_ID_WCCD eq_refl eq_refl from_addr to_addr amt.
+    Proof.
+      intros Haddr.
+      cbn in *.
+      destruct (AddressMap.find _ _) as [v |] eqn:Hv;try congruence.
+      destruct (requireTrue _) eqn:Heq;try congruence.
+      inversion Haddr;subst;clear Haddr.
+      destruct (amt <=? wccd_balance v) eqn:Hamt;cbn in *;try congruence.
+      apply leb_complete in Hamt.
+      repeat split;cbn.
+      + intros.
+        unfold setter_from_getter_AddressState_wccd_balance,set_AddressState_wccd_balance.
+        unfold WccdView.get_balance_opt, get_balance_opt.
+        rewrite inctement_balance_find_ne by assumption.
+        unfold AddressMap.find,AddressMap.add.
+        now erewrite fin_maps.lookup_insert_ne.
+      + intros. unfold setter_from_getter_AddressState_wccd_balance,set_AddressState_wccd_balance.
+        unfold WccdView.get_balance_opt, get_balance_opt.
+        unfold requireTrue in Heq.
+        destruct (_ =? _) eqn:Heq1;auto;cbn. now rewrite Nat.eqb_eq in Heq1.
+      + repeat rewrite get_balance_total_get_balance_default.
+        repeat unfold setter_from_getter_AddressState_wccd_balance,
+          set_AddressState_wccd_balance,increment_balance.
+        unfold get_balance_default,cis1_axioms.VExtra.get_balance in *. cbn.
+        unfold setter_from_getter_AddressState_wccd_balance,set_AddressState_wccd_balance.
+        destruct (AddressMap.find to_addr _) eqn:Haddr.
+        * unfold get_balance_opt,AddressMap.find,AddressMap.add in *.
+          rewrite Hv.
+          rewrite FMap.add_commute with (m:=prev_st) by auto.
+          rewrite FMap.find_add with (m:=(FMap.add _ _ prev_st));cbn.
+          lia.
+        * unfold get_balance_opt,AddressMap.find,AddressMap.add in *.
+          rewrite FMap.add_commute with (m:=prev_st) by auto.
+          rewrite FMap.find_add with (m:=(FMap.add _ _ prev_st)).
+          cbn. rewrite Hv. unfold requireTrue in Heq.
+          lia.
+      + repeat rewrite get_balance_total_get_balance_default.
+        repeat unfold setter_from_getter_AddressState_wccd_balance,
+          set_AddressState_wccd_balance,increment_balance.
+        unfold get_balance_default,cis1_axioms.VExtra.get_balance in *. cbn.
+        unfold setter_from_getter_AddressState_wccd_balance,set_AddressState_wccd_balance.
+        destruct (AddressMap.find to_addr _) eqn:Haddr.
+        * unfold get_balance_opt,AddressMap.find,AddressMap.add in *.
+          rewrite FMap.find_add with (m:=(FMap.add _ _ prev_st));cbn.
+          rewrite FMap.find_add_ne with (m:=prev_st) in Haddr by auto.
+          unfold FMap.find in *.
+          now rewrite Haddr.
+        * unfold get_balance_opt,AddressMap.find,AddressMap.add in *.
+          rewrite FMap.find_add with (m:=(FMap.add _ _ prev_st));cbn.
+          rewrite FMap.find_add_ne with (m:=prev_st) in Haddr by auto.
+          unfold FMap.find in *.
+          now rewrite Haddr.
+      + subst. repeat rewrite get_balance_total_get_balance_default.
+        repeat unfold setter_from_getter_AddressState_wccd_balance,
+          set_AddressState_wccd_balance,increment_balance.
+        unfold get_balance_default,cis1_axioms.VExtra.get_balance in *. cbn.
+        unfold setter_from_getter_AddressState_wccd_balance,set_AddressState_wccd_balance.
+        unfold get_balance_opt. now rewrite Hv.
+      + subst.
+        repeat rewrite get_balance_total_get_balance_default.
+        repeat unfold setter_from_getter_AddressState_wccd_balance,
+          set_AddressState_wccd_balance,increment_balance.
+        unfold get_balance_default,cis1_axioms.VExtra.get_balance in *. cbn.
+        unfold get_balance_opt.
+        rewrite Hv.
+        unfold AddressMap.find,AddressMap.add.
+        rewrite FMap.find_add with (m:=prev_st);cbn.
+        rewrite FMap.find_add with (m:=FMap.add _ _ prev_st);cbn.
+        lia.
+    Qed.
+
+    Definition contract_receive := wccd_receive.
+
+    Theorem receive_spec :
+    forall (chain : Chain)
+      (ctx : ContractCallContext)
+      (entry : CIS1_entry_points)
+      (msg : Msg)
+      (prev_st next_st : State)
+      (ops : list ActionBody),
+      get_CIS1_entry_point msg = Some entry ->
+      wccd_receive chain ctx prev_st (Some msg) = Some (next_st, ops) ->
+      match entry with
+      | CIS1_transfer params => transfer_spec params prev_st next_st ops
+      | CIS1_updateOperator params => updateOperator_spec ctx params prev_st next_st ops
+      | CIS1_balanceOf params => balanceOf_spec params prev_st next_st ops
+      end.
+    Proof.
+      intros ? ? ? ? ? ? ? Hep Hreceive.
+      destruct msg;cbn;inversion Hep;subst;clear Hep;try easy.
+      + simpl in *.
+        destruct (wccd_transfer _ _) eqn:Htr;try congruence.
+        inversion Hreceive;subst;clear Hreceive.
+        constructor.
+        * cbn.
+          revert dependent next_st.
+          revert dependent prev_st.
+          induction params.
+          ** cbn in *. congruence.
+          ** intros prev_st next_st Hreceive.
+             cbn -[wccd_transfer_single] in *.
+             destruct (wccd_transfer_single _ _ _ _ _) as [st |] eqn:Haddr;try congruence.
+             destruct a as [amt from_addr to_addr];cbn.
+             simpl in *.
+             exists st, eq_refl, eq_refl.
+             split.
+             *** cbn in *. now apply wccd_transfer_single_cis1.
+             *** now eapply IHparams.
+        * cbn.
+          revert dependent prev_st.
+          revert dependent next_st.
+          induction params.
+          ** intros;cbn;auto.
+          ** intros;cbn -[wccd_transfer_single] in *.
+             destruct (wccd_transfer_single _ _ _ _ _) as [st |] eqn:Haddr;try congruence.
+             destruct a as [amt from_addr to_addr];cbn.
+             destruct (address_is_contract _).
+             *** constructor;simpl in *.
+                 eexists. split.
+                 **** reflexivity.
+                 **** exists unit. eexists.
+                      apply deserialize_serialize.
+                 **** eapply IHparams;eauto.
+             *** eapply IHparams;eauto.
+      + simpl in *.
+        admit.
+      + admit.
+    Admitted.
+
+  End WccdReceiveDefs.
+End WccdReceiveSpec.
